SporkProofs/Soundness.lean
@@ -1,0 +1,44 @@
+import SporkProofs.Syntax
+import SporkProofs.Semantics
+import SporkProofs.Progress
+import SporkProofs.Preservation
+
+namespace Steps
+
+  theorem preservation {P : Program} (Pwf : P.WF) :
+                        {R R' : ThreadTree} ->
+                        R.WF P -> P ⊢ R ↦* R' -> R'.WF P
+    | R, .(R), Rwf, .nil => Rwf
+    | R, R'', Rwf, @Steps.cons .(P) .(R) R' .(R'') R_sR' R'_R'' =>
+      Step.preservation Pwf (preservation Pwf Rwf R_sR') R'_R''
+
+  theorem preserves_prom {P : Program} (Pwf : P.WF) : {R R' : ThreadTree} ->
+                         P ⊢ R ↦* R' -> R.WF P -> R.prom = R'.prom
+  | R, .(R), .nil, _Rwf  => rfl
+  | R, R'', @Steps.cons .(P) .(R) R' .(R'') R_R' R'_R'', Rwf =>
+    let p_R_R' : R.prom = R'.prom := preserves_prom Pwf R_R' Rwf
+    let p_R'_R'' : R'.prom = R''.prom := Step.preserve_prom R'_R'' (preservation Pwf Rwf R_R')
+    Eq.trans p_R_R' p_R'_R''
+
+  def soundness {P : Program} (Pwf : P.WF) {R R' : ThreadTree}
+                (Rwf : R.WF P) (R_R' : P ⊢ R ↦* R') : Step.Next P R' :=
+    Step.progress R' (preservation Pwf Rwf R_R')
+
+  inductive NextRoot (P : Program) : ThreadTree -> Type where
+    | result (g X x) :
+        NextRoot P {{⟨g, ∅, X, .code (.retn x)⟩}}
+    | step {R} (R') (s : P ⊢ R ↦ R') :
+        NextRoot P R
+
+  def program_soundness {P : Program} (Pwf : P.WF) {R : ThreadTree}
+                        (ss : P ⊢ (ThreadTree.init P) ↦* R) : NextRoot P R :=
+    let Piwf := ThreadTree.WF.init Pwf
+    let Rwf := preservation Pwf Piwf ss
+    match Step.progress R Rwf with
+      | .result g X x => .result g X x
+      | .blocked K f gret π X bunpr bprom =>
+        let c := preserves_prom Pwf ss Piwf
+        by contradiction
+      | .step R' s => .step R' s
+
+end Steps
